fairneris/aneris_lang/state_interp/state_interp_config_wp.v
@@ -41,115 +41,118 @@ Section state_interpretation.
 
   (* OBS: A general update lemma could be nicer, but needs changes to
    [network_sockets_coh] API *)
-  Lemma state_buffers_insert ip (skts : gmap ip_address sockets)
-        sh skt bs m R Sn sa :
-    network_sockets_coh skts →
-    m_destination m = sa →
-    ip = ip_of_address sa →
-    skts !! ip = Some Sn →
-    Sn !! sh = Some (skt, R) →
-    saddress skt = Some sa →
-    model_state_socket_coh skts bs →
-    model_state_socket_coh (<[ip:=<[sh:=(skt, m :: R)]> Sn]> skts)
-                           (<[sa:=m :: R]> bs).
-  Proof.
-    intros Hscoh Hm -> Hip Hsh Hsa Hcoh ip' Sn' sh' skt' sa' R' Hip' Hsh' Hskt'.
-    assert (network_sockets_coh (<[ip_of_address sa:=<[sh:=(skt, m :: R)]> Sn]> skts)) as Hscoh'.
-    { by eapply network_sockets_coh_deliver_message. }
-    assert (ip_of_address sa' = ip') as <-.
-    { by eapply Hscoh'. }
-    destruct (decide (sa = sa')) as [<-|Hsaneq].
-    { destruct sa.
-      rewrite lookup_total_insert.
-      rewrite lookup_insert in Hip'.
-      simplify_eq.
-      assert(sh = sh') as <-.
-      { eapply Hscoh'; [| |done|..].
-        - apply lookup_insert.
-        - rewrite lookup_insert. done.
-        - done.
-        - rewrite Hsa. rewrite Hskt'. done. }
-      rewrite lookup_insert in Hsh'.
-      simplify_eq. done. }
-    rewrite lookup_total_insert_ne; [|done].
-    destruct (decide (ip_of_address sa = ip_of_address sa')) as [Heq|Hneq].
-    { rewrite Heq in Hip'. rewrite lookup_insert in Hip'.
-      simplify_eq.
-      assert(sh ≠ sh') as Hshneq.
-      { intros <-. rewrite lookup_insert in Hsh'. simplify_eq. }
-      rewrite lookup_insert_ne in Hsh'; [|done].
-      by eapply Hcoh. }
-    rewrite lookup_insert_ne in Hip'; [|done].
-    by eapply Hcoh.
-  Qed.
+  (* Lemma state_buffers_insert ip (skts : gmap ip_address sockets) *)
+  (*       sh skt bs m R Sn sa : *)
+  (*   network_sockets_coh skts → *)
+  (*   m_destination m = sa → *)
+  (*   ip = ip_of_address sa → *)
+  (*   skts !! ip = Some Sn → *)
+  (*   Sn !! sh = Some (skt, R) → *)
+  (*   saddress skt = Some sa → *)
+  (*   model_state_socket_coh skts bs → *)
+  (*   model_state_socket_coh (<[ip:=<[sh:=(skt, m :: R)]> Sn]> skts) *)
+  (*                          (<[sa:=m :: R]> bs). *)
+  (* Proof. *)
+  (*   intros Hscoh Hm -> Hip Hsh Hsa Hcoh ip' Sn' sh' skt' sa' R' Hip' Hsh' Hskt'. *)
+  (*   assert (network_sockets_coh (<[ip_of_address sa:=<[sh:=(skt, m :: R)]> Sn]> skts)) as Hscoh'. *)
+  (*   { by eapply network_sockets_coh_deliver_message. } *)
+  (*   assert (ip_of_address sa' = ip') as <-. *)
+  (*   { by eapply Hscoh'. } *)
+  (*   destruct (decide (sa = sa')) as [<-|Hsaneq]. *)
+  (*   { destruct sa. *)
+  (*     rewrite lookup_total_insert. *)
+  (*     rewrite lookup_insert in Hip'. *)
+  (*     simplify_eq. *)
+  (*     assert(sh = sh') as <-. *)
+  (*     { eapply Hscoh'; [| |done|..]. *)
+  (*       - apply lookup_insert. *)
+  (*       - rewrite lookup_insert. done. *)
+  (*       - done. *)
+  (*       - rewrite Hsa. rewrite Hskt'. done. } *)
+  (*     rewrite lookup_insert in Hsh'. *)
+  (*     simplify_eq. done. } *)
+  (*   rewrite lookup_total_insert_ne; [|done]. *)
+  (*   destruct (decide (ip_of_address sa = ip_of_address sa')) as [Heq|Hneq]. *)
+  (*   { rewrite Heq in Hip'. rewrite lookup_insert in Hip'. *)
+  (*     simplify_eq. *)
+  (*     assert(sh ≠ sh') as Hshneq. *)
+  (*     { intros <-. rewrite lookup_insert in Hsh'. simplify_eq. } *)
+  (*     rewrite lookup_insert_ne in Hsh'; [|done]. *)
+  (*     by eapply Hcoh. } *)
+  (*   rewrite lookup_insert_ne in Hip'; [|done]. *)
+  (*   by eapply Hcoh. *)
+  (* Qed. *)
 
-  Lemma state_buffers_delete ip (skts : gmap ip_address sockets)
-        sh skt bs m R Sn sa :
-    network_sockets_coh skts →
-    m_destination m = sa →
-    ip = ip_of_address sa →
-    skts !! ip = Some Sn →
-    Sn !! sh = Some (skt, R ++ [m]) →
-    saddress skt = Some sa →
-    model_state_socket_coh skts bs →
-    model_state_socket_coh (<[ip:=<[sh:=(skt, R)]> Sn]> skts)
-                           (<[sa:=R]> bs).
-  Proof.
-    intros Hscoh Hm -> Hip Hsh Hsa Hcoh ip' Sn' sh' skt' sa' R' Hip' Hsh' Hskt'.
-    assert (network_sockets_coh (<[ip_of_address sa:=<[sh:=(skt, R)]> Sn]> skts)) as Hscoh'.
-    { by eapply network_sockets_coh_receive. }
-    assert (ip_of_address sa' = ip') as <-.
-    { by eapply Hscoh'. }
-    destruct (decide (sa = sa')) as [<-|Hsaneq].
-    { destruct sa.
-      rewrite lookup_total_insert.
-      rewrite lookup_insert in Hip'.
-      simplify_eq.
-      assert(sh = sh') as <-.
-      { eapply Hscoh'; [| |done|..].
-        - apply lookup_insert.
-        - rewrite lookup_insert. done.
-        - done.
-        - rewrite Hsa. rewrite Hskt'. done. }
-      rewrite lookup_insert in Hsh'.
-      simplify_eq. done. }
-    rewrite lookup_total_insert_ne; [|done].
-    destruct (decide (ip_of_address sa = ip_of_address sa')) as [Heq|Hneq].
-    { rewrite Heq in Hip'. rewrite lookup_insert in Hip'.
-      simplify_eq.
-      assert(sh ≠ sh') as Hshneq.
-      { intros <-. rewrite lookup_insert in Hsh'. simplify_eq. }
-      rewrite lookup_insert_ne in Hsh'; [|done].
-      by eapply Hcoh. }
-    rewrite lookup_insert_ne in Hip'; [|done].
-    by eapply Hcoh.
-  Qed.
+  (* Lemma state_buffers_delete ip (skts : gmap ip_address sockets) *)
+  (*       sh skt bs m R Sn sa : *)
+  (*   network_sockets_coh skts → *)
+  (*   m_destination m = sa → *)
+  (*   ip = ip_of_address sa → *)
+  (*   skts !! ip = Some Sn → *)
+  (*   Sn !! sh = Some (skt, R ++ [m]) → *)
+  (*   saddress skt = Some sa → *)
+  (*   model_state_socket_coh skts bs → *)
+  (*   model_state_socket_coh (<[ip:=<[sh:=(skt, R)]> Sn]> skts) *)
+  (*                          (<[sa:=R]> bs). *)
+  (* Proof. *)
+  (*   intros Hscoh Hm -> Hip Hsh Hsa Hcoh ip' Sn' sh' skt' sa' R' Hip' Hsh' Hskt'. *)
+  (*   assert (network_sockets_coh (<[ip_of_address sa:=<[sh:=(skt, R)]> Sn]> skts)) as Hscoh'. *)
+  (*   { by eapply network_sockets_coh_receive. } *)
+  (*   assert (ip_of_address sa' = ip') as <-. *)
+  (*   { by eapply Hscoh'. } *)
+  (*   destruct (decide (sa = sa')) as [<-|Hsaneq]. *)
+  (*   { destruct sa. *)
+  (*     rewrite lookup_total_insert. *)
+  (*     rewrite lookup_insert in Hip'. *)
+  (*     simplify_eq. *)
+  (*     assert(sh = sh') as <-. *)
+  (*     { eapply Hscoh'; [| |done|..]. *)
+  (*       - apply lookup_insert. *)
+  (*       - rewrite lookup_insert. done. *)
+  (*       - done. *)
+  (*       - rewrite Hsa. rewrite Hskt'. done. } *)
+  (*     rewrite lookup_insert in Hsh'. *)
+  (*     simplify_eq. done. } *)
+  (*   rewrite lookup_total_insert_ne; [|done]. *)
+  (*   destruct (decide (ip_of_address sa = ip_of_address sa')) as [Heq|Hneq]. *)
+  (*   { rewrite Heq in Hip'. rewrite lookup_insert in Hip'. *)
+  (*     simplify_eq. *)
+  (*     assert(sh ≠ sh') as Hshneq. *)
+  (*     { intros <-. rewrite lookup_insert in Hsh'. simplify_eq. } *)
+  (*     rewrite lookup_insert_ne in Hsh'; [|done]. *)
+  (*     by eapply Hcoh. } *)
+  (*   rewrite lookup_insert_ne in Hip'; [|done]. *)
+  (*   by eapply Hcoh. *)
+  (* Qed. *)
 
   Lemma config_wp_correct : ⊢ config_wp.
   Proof.
     rewrite /config_wp. iModIntro.
     iIntros (ex atr c lbl σ2 Hexvalid Hex Hstep) "(% & Hsi & Hlive & Hauth)".
     rewrite (last_eq_trace_ends_in ex c); [|done].
+    rewrite /aneris_state_interp.
     iDestruct "Hsi" as (γm mh)
                          "(%Hhist & %Hgcoh & %Hnscoh & %Hmhcoh &
                            Hnauth & Hsi & Hlcoh & Hfreeips & Hmctx & Hmres)".
     iMod (steps_auth_update_S with "Hauth") as "Hauth".
     iApply fupd_elim_laterN; [solve_ndisj|].
     destruct c as [tp1 σ1]=> /=.
-    rewrite /simple_valid_state_evolution in H.
+    rewrite /valid_state_evolution_fairness in H.
     rewrite /trace_ends_in in Hex.
-    rewrite Hex in H. simpl in *.
     destruct σ1; simpl in *; simplify_eq.
-    destruct (trace_last atr) as [[δ ms] bs] eqn:Hs.
+    pose (trace_last atr) as δ.
     inversion Hstep as
       [ip σ Sn Sn' sh a skt R m Hm HSn Hsh HSn' Hsaddr|
         σ|
         σ];
       simplify_eq/=.
     (* Deliver *)
-    - destruct H as (Hsteps & Hmatch & Hlive & Hσ).
-      iExists (δ, ms ∖ {[+ m +]}, <[m_destination m := m::R]>bs),
-                (inr ((), Some m)).
+    - destruct H as (Hsteps & Hmatch & Htids & Hsm).
+      destruct (LM.(lm_cfg_action) (trace_last atr) (Some m)) as [ℓ δ'].
+      unshelve iExists ({| ls_data := {| ls_under := δ'; ls_map := δ.(ls_data).(ls_map) |} |}).
+      { admit. }
+      { admit. }
+      iExists (Config_step ℓ (Some m : config_label aneris_lang)).
       iSplitR.
       { iPureIntro.
         rewrite /simple_valid_state_evolution.
